appendixA/coq/typing.v
@@ -1,0 +1,1049 @@
+
+(*
+
+This file contains the coq formalization
+of section Appendix A of thesis.
+
+-> Contains properties of preservation,
+   progress, and determinism.
+
+-> Revised Dsijointness Algorithm with COST
+
+*)
+
+Require Import TLC.LibLN.
+Require Import Program.Equality.
+Require Import Coq.Lists.ListSet.
+From Coq Require Export Lists.List.
+Export ListNotations.
+(* Require Import Coq.Strings.String. *)
+
+Require Import syntax.
+
+(** definitions *)
+
+(* defns value *)
+Inductive value : exp -> Prop :=    (* defn value *)
+ | val_int : forall i5,
+     value (e_lit i5)
+ | val_abs : forall e,
+     lc_exp (e_abs e) ->
+     value (e_abs e)
+ | val_null :
+     value e_null.
+
+(* defns FindType *)
+Inductive findtype : exp -> typ -> Prop :=    (* defn findtype *)
+ | findtype_int : forall i5,
+     findtype (e_lit i5) t_int
+ | findtype_arrow : forall (e:exp),
+     lc_exp (e_abs e) ->
+     findtype  (e_abs e) (t_arrow t_top t_bot)
+ | findtype_null :
+     findtype e_null t_unit.
+
+#[export]
+Hint Constructors value findtype : core.
+
+(****** Counting Free Variables ******)
+
+(** Computing free term variables in a type *)
+
+Fixpoint fv_ee (e : exp) {struct e} : vars :=
+  match e with
+  | e_bvar i    => \{}
+  | e_fvar x    => \{x}
+  | e_lit i     => \{}
+  | e_abs e    => (fv_ee e)
+  | e_app e1 e2 => (fv_ee e1) \u (fv_ee e2)
+  | e_typeof e A e1 B e2 => (fv_ee e) \u (fv_ee e1) \u (fv_ee e2)
+  | e_null      => \{}
+  end.
+
+(***** Substitution Functions ******)
+
+(** Substitution for free type variables in types. *)
+
+
+(** Substitution for free term variables in terms. *)
+
+Fixpoint subst_ee (z : var) (u : exp) (e : exp) {struct e} : exp :=
+  match e with
+  | e_bvar i    => e_bvar i
+  | e_fvar x    => If (x = z) then u else e_fvar x
+  | e_lit i     => e_lit i 
+  | e_abs e    => e_abs (subst_ee z u e)
+  | e_app e1 e2 => e_app (subst_ee z u e1) (subst_ee z u e2)
+  | e_typeof e A e1 B e2 => e_typeof (subst_ee z u e) A (subst_ee z u e1) B (subst_ee z u e2)
+  | e_null      => e_null
+  end.
+
+
+(* defns Typing *)
+Reserved Notation "G |= e : A" (at level 80, e at next level, A at next level).
+Inductive typing : env -> exp -> typ -> Prop :=    (* defn typing *)
+ | typ_lit : forall (G:env) i5,
+      okt G  ->
+     typing G (e_lit i5) t_int
+ | typ_null : forall G,
+      okt G ->
+      typing G e_null t_unit
+ | typ_var : forall (G:env) (x:var) (A:typ),
+      okt G ->
+      binds x (bind_typ A) G  ->
+      typing G (e_fvar x) A
+ | typ_app : forall (G:env) (e1 e2:exp) (B A:typ),
+     typing G e1 (t_arrow A B) ->
+     typing G e2 A ->
+     typing G (e_app e1 e2) B
+ | typ_sub : forall (G:env) (e:exp) (A B:typ),
+     typing G e B ->
+     sub B A ->
+     typing G e A
+ | typ_abs : forall (L:vars) (G:env) (e:exp) (A B:typ),
+      okt G ->
+      ( forall x , x \notin  L  -> typing (G & x ~: A) (open_ee e (e_fvar x)) B)  ->
+     typing G (e_abs e) (t_arrow A B)
+ | typ_typeof : forall (L:vars) (G:env) (e:exp) (A:typ) (e1:exp) (B:typ) (e2:exp) (C:typ),
+     typing G e (t_union A B) ->
+     ( forall x ,x \notin  L -> typing (G & x ~: A ) (open_ee e1 (e_fvar x) ) C) ->
+     ( forall x ,x \notin  L -> typing (G & x ~: B ) (open_ee e2 (e_fvar x) ) C) ->
+     A *s B ->
+     typing G (e_typeof e A e1 B e2) C
+ | typ_inter : forall G e A B,
+     typing G e A ->
+     typing G e B ->
+     typing G e (t_and A B)
+where "G |= e : A" := (typing G e A).
+
+
+(* defns Reduction *)
+Reserved Notation "e --> e'" (at level 80, e' at next level).
+Inductive step : exp -> exp -> Prop :=    (* defn step *)
+ | step_appl : forall (e1 e2 e1':exp),
+     lc_exp e2 ->
+     step e1 e1' ->
+     step (e_app e1 e2) (e_app e1' e2)
+ | step_appr : forall (v e e':exp),
+     value v ->
+     step e e' ->
+     step (e_app v e) (e_app v e')
+ | step_beta : forall (e:exp) (v:exp),
+     lc_exp (e_abs e) ->
+     value v ->
+     step (e_app (e_abs e) v) (open_ee e v)
+ | step_typeof : forall (e:exp) (A:typ) (e1:exp) (B:typ) (e2 e':exp),
+     lc_exp (e_typeof e A e1 B e2) ->
+     step e e' ->
+     step (e_typeof e A e1 B e2) (e_typeof e' A e1 B e2)
+ | step_typeofl : forall (v:exp) (A:typ) (e1:exp) (B:typ) (e2:exp) (C:typ),
+     lc_exp (e_typeof v A e1 B e2) ->
+     value v ->
+     findtype v C ->
+     sub C A ->
+     step (e_typeof v A e1 B e2) (open_ee e1 v)
+ | step_typeofr : forall (v:exp) (A:typ) (e1:exp) (B:typ) (e2:exp) (C:typ),
+    lc_exp (e_typeof v A e1 B e2) ->
+     value v ->
+     findtype v C ->
+     sub C B ->
+     step (e_typeof v A e1 B e2) (open_ee  e2 v )
+where "e --> e'" := (step e e') : env_scope.
+
+#[export]
+Hint Constructors typing step : core.
+
+(** Gathering free names already used in the proofs **)
+
+Ltac gather_vars :=
+  let A := gather_vars_with (fun x : vars => x) in
+  let B := gather_vars_with (fun x : var => \{x}) in
+  let C := gather_vars_with (fun x : exp => fv_ee x) in
+  let D := gather_vars_with (fun x : env => dom x) in
+  constr:(A \u B \u C \u D).
+
+(** "pick_fresh x" tactic create a fresh variable with name x *)
+
+Ltac pick_fresh x :=
+  let L := gather_vars in (pick_fresh_gen L x).
+
+(** "apply_fresh T as x" is used to apply inductive rule which
+   use an universal quantification over a cofinite set *)
+
+Tactic Notation "apply_fresh" constr(T) "as" ident(x) :=
+  apply_fresh_base T gather_vars x.
+
+Tactic Notation "apply_fresh" "*" constr(T) "as" ident(x) :=
+  apply_fresh T as x; autos*.
+
+(** These tactics help applying a lemma which conclusion mentions
+  an environment (E & F) in the particular case when F is empty *)
+
+Ltac get_env :=
+  match goal with
+  | |- sub _ ?E _ _  => E
+  | |- typing _ ?E _ _ => E
+  end.
+
+Tactic Notation "apply_empty_bis" tactic(get_env) constr(lemma) :=
+  let E := get_env in rewrite <- (concat_empty_r E);
+  eapply lemma; try rewrite concat_empty_r.
+
+Tactic Notation "apply_empty" constr(F) :=
+  apply_empty_bis (get_env) F.
+
+Tactic Notation "apply_empty" "*" constr(F) :=
+  apply_empty F; autos*.
+
+(** Tactic to undo when Coq does too much simplification *)
+
+(* ********************************************************************** *)
+(** * Properties of Substitutions *)
+
+
+(** Substitution for a fresh name is identity. *)
+
+(** Substitution and open_var for distinct names commute. *)
+
+
+(* ********************************************************************** *)
+(** ** Properties of term substitution in terms *)
+
+Lemma open_ee_rec_term_core : forall e j v u i, i <> j ->
+open_ee_rec j v e = open_ee_rec i u (open_ee_rec j v e) ->
+  e = open_ee_rec i u e.
+Proof.
+  induction e; introv Neq H; simpl in *; inversion H; f_equal*.
+  case_nat*. case_nat*.
+Qed.
+
+
+Lemma open_ee_rec_term : forall u e,
+  lc_exp e -> forall k, e = open_ee_rec k u e.
+Proof.
+  induction 1; intros; simpl; f_equal*.
+  unfolds open_ee_rec. pick_fresh x.
+   apply* (@open_ee_rec_term_core e 0 (e_fvar x)).
+  unfolds open_ee. pick_fresh x.
+   apply* (@open_ee_rec_term_core e1 0 (e_fvar x)).
+  unfolds open_ee. pick_fresh x.
+   apply* (@open_ee_rec_term_core e2 0 (e_fvar x)).
+Qed.
+
+(** Substitution for a fresh name is identity. *)
+
+Lemma subst_ee_fresh : forall x u e,
+  x \notin fv_ee e -> subst_ee x u e = e.
+Proof.
+  induction e; simpl; intros; f_equal*.
+  case_var*.
+Qed.
+
+(** Substitution distributes on the open operation. *)
+
+Lemma subst_ee_open_ee : forall t1 t2 u x, lc_exp u ->
+subst_ee x u (open_ee t1 t2) =
+open_ee (subst_ee x u t1) (subst_ee x u t2).
+Proof.
+  intros. unfold open_ee. generalize 0.
+  induction t1; intros; simpls; f_equal*.
+  case_nat*.
+  case_var*. rewrite* <- open_ee_rec_term.
+Qed.
+
+(** Substitution and open_var for distinct names commute. *)
+
+Lemma subst_ee_open_ee_var : forall x y u e, y <> x -> lc_exp u ->
+  (subst_ee x u e) open_ee_var y = subst_ee x u (e open_ee_var y).
+Proof.
+  introv Neq Wu. rewrite* subst_ee_open_ee.
+  simpl. case_var*.
+Qed.
+
+(** Opening up a body t with a type u is the same as opening
+  up the abstraction with a fresh name x and then substituting u for x. *)
+
+Lemma subst_ee_intro : forall x u e,
+  x \notin fv_ee e -> lc_exp u ->
+  open_ee e u = subst_ee x u (e open_ee_var x).
+Proof.
+  introv Fr Wu. rewrite* subst_ee_open_ee.
+  rewrite* subst_ee_fresh. simpl. case_var*.
+Qed.
+
+Lemma subst_ee_term : forall e1 Z e2,
+lc_exp e1 -> lc_exp e2 -> lc_exp (subst_ee Z e2 e1).
+Proof.
+  induction 1; intros; simpl; auto.
+  case_var*.
+ - apply_fresh* lc_e_abs as y.
+   rewrite* subst_ee_open_ee_var.
+ - apply_fresh* lc_e_typeof as y.
+   rewrite* subst_ee_open_ee_var.
+   rewrite* subst_ee_open_ee_var.
+Qed.
+
+#[export]
+Hint Resolve subst_ee_term : core.
+
+(* ********************************************************************** *)
+(** * Relations between well-formed environment and types well-formed
+  in environments *)
+
+(** If an environment is well-formed, then it does not contain duplicated keys. *)
+
+Lemma ok_from_okt : forall E,
+  okt E -> ok E.
+Proof.
+  induction 1. auto. auto.
+Qed.
+
+#[export]
+Hint Extern 1 (ok _) => apply (ok_from_okt _) : core.
+
+
+Lemma append_empty_right : forall (E : env),
+  E = E & empty.
+Proof.
+  intros.
+  rewrite~ concat_empty_r.
+Qed.
+
+(** Automation *)
+
+(* ********************************************************************** *)
+(** ** Properties of well-formedness of an environment *)
+
+(** Through type substitution *)
+
+(** Inversion lemma *)
+
+Lemma okt_push_inv : forall E x T,
+  okt (E & x ~: T) -> okt E /\ x # E.
+Proof.
+  introv O. inverts O.
+    false* empty_push_inv.
+    lets (?&M&?): (eq_push_inv H). inverts M. subst. autos.
+Qed.
+
+#[export]
+Hint Resolve okt_push_inv : core.
+
+(** Through strengthening *)
+
+Lemma okt_strengthen : forall x T (E F : env),
+  okt (E & x ~: T & F) ->
+  okt (E & F).
+Proof.
+  introv O. induction F using env_ind.
+  rewrite concat_empty_r in *. apply okt_push_inv in O. destruct~ O.
+  rewrite concat_assoc in *.
+  destruct v.
+  apply okt_push_inv in O. destructs O.
+  apply okt_typ; auto.
+Qed.
+
+Lemma okt_concat_inv : forall E F x V,
+  okt (E & (x ~: V) & F) -> okt E /\ x # E.
+Proof.
+  intros E F. gen E.
+  induction F using env_ind; introv; rew_env_concat; auto; introv ok.
+  apply okt_push_inv in ok.
+  destruct ok; auto.
+  destruct v.
+  apply okt_push_inv in ok.
+  destruct ok.
+  forwards*: IHF.
+Qed.
+
+
+(** Automation *)
+
+#[export]
+Hint Immediate okt_strengthen : core.
+
+(* ********************************************************************** *)
+(** ** Regularity of relations *)
+
+Lemma typing_regular : forall E e T,
+  typing E e T -> okt E /\ lc_exp e.
+Proof.
+  induction 1; try splits*.
+ - (*case abs*)
+   apply lc_e_abs with (L:=L). intros.
+   specializes H1 x. destructs~ H1.
+ - (*case typeof*)
+   apply lc_e_typeof with (L:=L); intros. destructs~ IHtyping.
+   destructs~ IHtyping.
+   forwards*: H1 x.
+   destructs~ IHtyping.
+   forwards*: H3 x.
+Qed.
+
+(** The value relation is restricted to well-formed objects. *)
+
+Lemma value_regular : forall t,
+  value t -> lc_exp t.
+Proof.
+  induction 1; autos*.
+Qed.
+
+#[export]
+Hint Immediate value_regular : core.
+
+(** The reduction relation is restricted to well-formed objects. *)
+
+Lemma step_regular : forall t t',
+  step t t' -> lc_exp t /\ lc_exp t'.
+Proof.
+  induction 1; split*.
+  - inverts H. pick_fresh y. rewrite* (@subst_ee_intro y).
+  - inverts H. destructs IHstep.
+    apply_fresh* lc_e_typeof as y.
+  - inverts H. pick_fresh y. rewrite* (@subst_ee_intro y).
+  - inverts H. pick_fresh y. rewrite* (@subst_ee_intro y).
+Qed.
+
+(** Automation *)
+
+#[export]
+Hint Extern 1 (okt ?E) =>
+  match goal with
+  | H: typing _ _ _ |- _ => apply (proj31 (typing_regular H))
+  end : core.
+
+#[export]
+Hint Extern 1 (lc_exp ?e) =>
+  match goal with
+  | H: typing _ ?e _ |- _ => apply (proj32 (typing_regular H))
+  | H: step ?e _ |- _ => apply (proj1 (step_regular H))
+  | H: step _ ?e |- _ => apply (proj2 (step_regular H))
+  end : core.
+
+Lemma demorgan2 : forall P Q, ~ (P \/ Q) -> ~P /\ ~Q.
+Proof.
+  unfold not in *; intros.
+  splits; intros.
+  apply H; auto.
+  apply H; auto.
+Qed.
+
+
+(* ********************************************************************** *)
+(** Typing Weakening *)
+
+Lemma typing_weakening : forall E F G e T,
+   typing (E & G) e T ->
+   okt (E & F & G) ->
+   typing (E & F & G) e T.
+Proof.
+  introv Typ. gen F. inductions Typ; introv Ok.
+  - apply* typ_lit.
+  - apply* typ_null.
+  - apply* typ_var. 
+    apply* binds_weaken.
+  - apply* typ_app.
+  - apply* typ_sub.
+  - pick_fresh y.
+    apply typ_abs with (L:=L \u fv_ee e
+       \u dom E \u dom G \u dom F); auto.
+    intros.
+    forwards~: (H0 x).
+    apply_ih_bind (H1 x); eauto.
+  - pick_fresh y.
+    apply typ_typeof with (L:=L \u fv_ee e 
+       \u dom E \u dom G \u dom F); intros; autos*.
+    + forwards* : H x. apply_ih_bind (H0 x); eauto.
+    + forwards* : H1 x. apply_ih_bind (H2 x); eauto.
+  - apply* typ_inter.
+Qed.
+
+
+(************************************************************************ *)
+(** Preservation by Type Narrowing *)
+
+(************************************************************************ *)
+(** Preservation by Term Substitution (8) *)
+
+Lemma typing_through_subst_ee : forall E F x T e u U,
+   typing (E & x ~: U & F) e T ->
+   typing E u U ->
+   typing (E & F) (subst_ee x u e) T.
+Proof.
+introv TypT TypU.
+lets TypT': TypT.
+inductions TypT; simpl.
+(*case int*)
+ - apply* typ_lit.
+ - (*case null*)
+   apply* typ_null.
+(*case var*)
+ - case_var.
+  + binds_get H0.
+    (* apply ok_from_okt in H; auto. *)
+    lets M: (typing_weakening E F empty u U).
+    do 2 rewrite concat_empty_r in M.
+    apply* M.
+  + binds_cases H0; apply* typ_var.
+(*case app*)
+ - eapply typ_app; eauto.
+(*case sub*)
+ - forwards* : IHTypT E F TypU TypT.
+(*case abs*)
+ - pick_fresh y.
+   apply typ_abs with (L:=L \u \{ x} \u fv_ee u 
+     \u fv_ee e \u dom E \u dom F); intros; autos*.
+   assert (x0 \notin L) by auto.
+   specialize (H1 x0 H3 E (F & x0 ~: A)).
+   rewrite* subst_ee_open_ee_var.
+   lets : H1 x U.
+   forwards* : H4.
+   rewrite~ concat_assoc.
+   rewrite~ concat_assoc.
+   rewrite~ <- concat_assoc.
+   apply typing_regular in TypU. destructs~ TypU.
+(*case typeof*)
+ - pick_fresh y.
+   apply typ_typeof with (L:=L \u \{ x} \u fv_ee u 
+     \u fv_ee e \u fv_ee e1 \u fv_ee e2 \u
+      dom E \u dom F); intros; eauto.
+ + rewrite* subst_ee_open_ee_var.
+   forwards*: H x0.
+   forwards*: H0 x0 E (F & x0 ~: A) x.
+   rewrite~ concat_assoc.
+   rewrite~ concat_assoc.
+   rewrite~ <- concat_assoc.
+   apply typing_regular in TypU. destructs~ TypU.
+ + rewrite* subst_ee_open_ee_var.
+   forwards*: H1 x0.
+   forwards*: H2 x0 E (F & x0 ~: B) x.
+   rewrite~ concat_assoc.
+   rewrite~ concat_assoc.
+   rewrite~ <- concat_assoc.
+   apply typing_regular in TypU. destructs~ TypU.
+- apply* typ_inter.
+Qed.
+
+
+Lemma UO_sub_union : forall B B1 B2,
+  US B B1 B2 ->
+  forall A, UO A ->
+  sub A B ->
+  sub A B1 \/ sub A B2.
+Proof.
+  induction 1;
+  introv Ord Sub.
+  induction Ord; inverts* Sub.
+  1,2: apply sub_and in Sub;
+       forwards*: IHUS Ord.
+Qed.
+
+Require Import Lia.
+
+Lemma US_size_red : forall A A1 A2,
+  US A A1 A2 -> t_size A1 < t_size A /\ t_size A2 < t_size A.
+Proof.
+  induction 1; intros; simpl. lia.
+  destruct IHUS. split. lia. lia.
+  destruct IHUS. split. lia. lia.
+Defined.
+
+(* ********************************************************************** *)
+(** Preservation Result (20) *)
+
+Lemma inv_int : forall E A i5,
+typing E (e_lit i5) A -> typing E (e_lit i5) t_int /\ sub t_int A.
+Proof.
+  introv Typ.
+  inductions Typ.
+  (*case typ_int*)
+ - split*.
+  (*case typ_sub*)
+ - specialize (IHTyp i5).
+  forwards* : IHTyp. destruct H0.
+  split*.
+  eapply sub_transitivity; eauto.
+  - forwards* : IHTyp1. destruct H.
+    forwards* : IHTyp2.
+Qed.
+
+Lemma abs_typ_arrow_sub : forall G e A,
+typing G (e_abs e) A ->
+exists A1 B1, sub (t_arrow A1 B1) A.
+Proof.
+    introv Typ.
+    inductions Typ.
+    - forwards* : IHTyp. destruct H0 as [x1[x2 H3]].
+      exists x1 x2. eapply sub_transitivity; eauto.
+    - exists* A B.
+    - forwards* : IHTyp1.
+      forwards* : IHTyp2.
+      destruct H as [x1 [x2 H3]].
+      destruct H0 as [x3 [x4 H4]].
+      exists t_top t_bot.
+      apply s_anda.
+      assert (sub (t_arrow t_top t_bot) (t_arrow x1 x2)); eauto.
+      eapply sub_transitivity; eauto.
+      assert (sub (t_arrow t_top t_bot) (t_arrow x3 x4)); eauto.
+      eapply sub_transitivity; eauto.
+Qed.
+
+Lemma inv_and_arrow : forall G e A1 A2 B1 B2,
+  typing G (e_abs e) (t_and A1 A2) ->
+  sub (t_and A1 A2) (t_arrow B1 B2) ->
+  sub A1 (t_arrow B1 B2) \/ sub A2 (t_arrow B1 B2).
+Proof.
+  introv Typ Sub.
+  inverts Sub; eauto.
+Qed.
+
+Lemma inv_abs_sub : forall G e A B1 B2,
+    typing G (e_abs e) A ->
+    sub A (t_arrow B1 B2) ->
+         exists C1 C2,
+           (exists L, forall x , x \notin  L -> typing (G & x ~: C1) (e open_ee_var x) C2)
+           /\ sub (t_arrow C1 C2) (t_arrow B1 B2).
+Proof.
+  introv Typ Sub.
+  inductions Typ; eauto.
+  - assert (HS: sub B (t_arrow B1 B2)) by applys sub_transitivity H Sub.
+    forwards* (?&?&?&?): IHTyp HS.
+  - forwards* [HS|HS]: inv_and_arrow Sub.
+Qed.
+
+
+Lemma inv_arrow : forall G e A1 A2,
+    typing G (e_abs e) (t_arrow A1 A2) ->
+    exists B1 B2, (exists L, forall x , x \notin  L -> typing (G & x ~: B1) (e open_ee_var x) B2)
+                  /\ sub (t_arrow B1 B2) (t_arrow A1 A2).
+Proof.
+  introv Typ.
+  inverts Typ.
+  - forwards* : inv_abs_sub H.
+  - exists A1 A2. split*.
+Qed.
+
+
+Lemma inv_abs_union : forall G e A A1 A2,
+    typing G (e_abs e) A ->
+    sub A (t_union A1 A2) ->
+    typing G (e_abs e) A1 \/ typing G (e_abs e) A2.
+Proof.
+  introv Typ Sub.
+  inductions Typ; eauto.
+  - eapply sub_transitivity in Sub; eauto.
+  - inverts* Sub.
+  - inverts* Sub.
+Qed.
+
+Lemma inv_null : forall E A,
+typing E e_null A -> typing E e_null t_unit /\ sub t_unit A.
+Proof.
+  introv Typ.
+  inductions Typ.
+  (*case typ_int*)
+ - split*.
+  (*case typ_sub*)
+ - forwards* : IHTyp. destruct H0.
+   split*.
+   eapply sub_transitivity; eauto.
+ - forwards* : IHTyp1.
+Qed.
+
+(*
+e = \x.x
+\x.x : (Int -> Int) /\ (Bool -> Bool) | (Int -> Int) /\ (Bool -> Bool)
+
+\x.x : (Int -> Int) /\ (Bool -> Bool)
+\x.x : (Int -> Int) /\ (Bool -> Bool)
+*)
+
+Lemma check_or_typ : forall E e A B,
+   value e ->
+   typing E e (t_union A B) ->
+   typing E e A \/ typing E e B.
+Proof.
+  introv Val Typ.
+  inverts Val.
+  (*subsumption again*)
+ - apply inv_int in Typ. destruct Typ.
+   inverts* H0.
+ - inverts Typ.
+   eapply inv_abs_union in H0; eauto.
+ - apply inv_null in Typ. destruct Typ.
+   inverts* H0.
+Qed.
+
+Lemma uord_sub_union : forall B B1 B2,
+  US B B1 B2 ->
+  forall A, Ord A ->
+  sub A B ->
+  sub A B1 \/ sub A B2.
+Proof.
+  induction 1;
+  introv Ord Sub.
+  inverts Ord; inverts* Sub.
+  1,2: apply sub_and in Sub;
+       forwards*: IHUS Ord.
+Qed.
+
+Lemma sub_ord_disjoint_types : forall A B,
+  A *s B ->
+  forall C, Ord C ->
+  sub C A ->
+  sub C B -> False.
+Proof.
+  introv Disj Ord SubA SubB.
+  unfold DisjSpec in Disj.
+  unfold not in Disj.
+  forwards*: Disj C.
+Qed.
+
+
+(********************************************************)
+(** A value cannot check against disjoint types **)
+
+Lemma val_check_disjoint_types : forall E v A B,
+  A *s B ->
+  value v ->
+  typing E v A ->
+  typing E v B -> False.
+Proof.
+  introv Disj Val Typ1 Typ2.
+  inverts Val.
+  - apply inv_int in Typ1. destruct Typ1.
+    apply inv_int in Typ2. destruct Typ2.
+    forwards*: sub_ord_disjoint_types Disj H0 H2.
+  - apply abs_typ_arrow_sub in Typ1.
+    destruct Typ1 as [A1 [B1]].
+    assert (sub (t_arrow t_top t_bot) (t_arrow A1 B1)); auto.
+    apply abs_typ_arrow_sub in Typ2.
+    destruct Typ2 as [A2 [B2]].
+    assert (sub (t_arrow t_top t_bot) (t_arrow A2 B2)); auto.
+    eapply sub_transitivity with (A:=(t_arrow t_top t_bot)) (B:=(t_arrow A1 B1)) (C:=A) in H1; auto.
+    eapply sub_transitivity with (A:=(t_arrow t_top t_bot)) (B:=(t_arrow A2 B2)) (C:=B) in H3; auto.
+    forwards*: sub_ord_disjoint_types Disj H1 H3.
+  - apply inv_null in Typ1. destruct Typ1.
+    apply inv_null in Typ2. destruct Typ2.
+    forwards*: sub_ord_disjoint_types Disj H0 H2.
+Qed.
+
+(*******************************************************)
+(** findtype gives least type of an expressions **)
+
+Lemma check_find_type : forall E e A B,
+typing E e A ->
+findtype e B ->
+sub B A.
+Proof.
+  introv Typ Find.
+  inductions Find.
+  - apply inv_int in Typ.
+    destruct~ Typ.
+  - apply abs_typ_arrow_sub in Typ.
+    destruct Typ as [A1 [B1]].
+    assert (sub (t_arrow t_top t_bot) (t_arrow A1 B1)) by auto.
+    eapply sub_transitivity; eauto.
+  - apply inv_null in Typ. destruct~ Typ.
+Qed.
+
+(********************************************)
+(** Values have ordinary types **)
+
+Lemma findtype_ord_type : forall v A,
+  findtype v A ->
+  Ord A.
+Proof.
+  introv Find.
+  inverts* Find.
+Qed.
+
+(*******************************)
+(****  Preservation Lemma  *****)
+(*******************************)
+
+Lemma preservation : forall E e e' T,
+  typing E e T ->
+  step e e' ->
+  typing E e' T.
+Proof.
+  introv Typ. gen e'.
+  induction Typ; introv Red; try solve [ inverts* Red ].
+  - (* app *)
+    inverts* Red.
+    (* beta *)
+        forwards* : inv_arrow Typ1.
+        destruct H as [A1[B1 [H H']]]. 
+        destruct H as [L].
+        pick_fresh x.
+        assert (x \notin L) by auto.
+        lets: H x H0.
+        assert (G & x ~: A1 = G & x ~: A1 & empty).
+        rewrite* concat_empty_r.
+        rewrite H4 in H2.
+        assert (G = G & empty).
+        rewrite* concat_empty_r. rewrite H5.
+        lets: typing_through_subst_ee.
+        inverts H'.
+        forwards* : H6 H2.
+        rewrite* (@subst_ee_intro x).
+  - (* typeof *)
+    inverts* Red.
+    
+    + (* value checks against disjoint types *)
+      lets temp: check_or_typ G e A B H11.
+      lets DisjOr: temp Typ.
+      destruct DisjOr.
+     * (*true goal*)
+       pick_fresh y. assert (y \notin L) by auto.
+       forwards* : H H5.
+       assert  (G & y ~: A = G & y ~: A & empty).
+       rewrite* concat_empty_r. rewrite H7 in H6.
+       assert (G = G & empty).
+       rewrite* concat_empty_r.
+       rewrite H8.
+       forwards* : typing_through_subst_ee.
+       rewrite* (@subst_ee_intro y).
+     * (*false goal, value e checks against disjoint types A and B*)
+       lets temp1: check_find_type G e B C0 H4.
+       lets SubB: temp1 H12.
+       inverts H12;
+       forwards*: sub_ord_disjoint_types H3 H13 SubB.
+    +  (* value checks against disjoint types *)
+      lets temp: check_or_typ G e A B H11.
+      lets DisjOr: temp Typ.
+      destruct DisjOr.
+     * (*false goal, value e checks against disjoint types A and B*)
+        lets temp1: check_find_type G e A C0 H4.
+        lets SubA: temp1 H12.
+        inverts H12;
+        forwards*: sub_ord_disjoint_types H3 SubA H13.
+     * (*true goal*)
+        pick_fresh y. assert (y \notin L) by auto.
+        forwards* : H1 H5.
+        assert  (G & y ~: B = G & y ~: B & empty).
+        rewrite* concat_empty_r. rewrite H7 in H6.
+        assert (G = G & empty).
+        rewrite* concat_empty_r.
+        rewrite H8.
+        forwards* : typing_through_subst_ee.
+        rewrite* (@subst_ee_intro y).
+    - forwards* : IHTyp1.
+Qed.
+
+
+(*******************************)
+(******  Progress Lemma  *******)
+(*******************************)
+
+Lemma progress : forall e T,
+typing empty e T -> (value e) \/ (exists e', step e e').
+Proof.
+introv Typ. gen_eq E: (@empty typ). lets Typ': Typ.
+inductions Typ; intros EQ; subst.
+(*case int*)
+ - left*.
+ (*case null*)
+ - left*.
+ (*case var*)
+ - apply binds_empty_inv in H0. inversion H0.
+ (*case typ-app*)
+ -  right. forwards* : IHTyp1.
+   destruct H.
+  + forwards* : IHTyp2.
+    destruct H0.
+   * inverts* H.
+     (*i infers arrow*)
+     apply inv_int in Typ1.
+     destruct Typ1.
+     inverts H1.
+     apply inv_null in Typ1.
+     destruct Typ1.
+     inverts H1.
+     (*case step-appl*)
+   * destruct H0.
+     exists* (e_app e1 x).
+   (*case step-appr*)
+  + destruct H.
+    exists (e_app x e2). apply* step_appl.
+    forwards* : typing_regular Typ2.
+(*case typ-sub*)
+ - forwards* : IHTyp.
+(*case typ-abs*)
+ - left. forwards* : typing_regular Typ'.
+(*case typ-typeof*)
+ - right. forwards* : IHTyp. 
+   destruct H4.
+  + apply check_or_typ in Typ; auto.
+    destruct Typ.
+    (*case typeofl*)
+   * destruct H4.
+     { (*case e = int*)
+      apply inv_int in H5. destruct H5.
+      exists (open_ee e1 (e_lit i5)).
+      pick_fresh y.
+      assert (y \notin L) by auto.
+      lets: H y H6.
+      eapply step_typeofl with (C:=t_int); eauto.
+      forwards* : typing_regular Typ'.
+     }
+     { (*case e = \x.e*)
+      apply abs_typ_arrow_sub in H5.
+      destruct H5 as [A1 [B1]].
+      assert (sub (t_arrow t_top t_bot) (t_arrow A1 B1)) by auto.
+      eapply sub_transitivity in H5; eauto.
+      exists (open_ee e1 (e_abs e)).
+      pick_fresh y.
+      forwards*: H y.
+      eapply step_typeofl with (C:=(t_arrow t_top t_bot)); eauto.
+      forwards* : typing_regular Typ'.
+     }
+     {
+       (*case e = null*)
+       apply inv_null in H5. destruct H5.
+       exists (open_ee e1 e_null).
+       pick_fresh y.
+       assert (y \notin L) by auto.
+       lets: H y H6.
+       eapply step_typeofl with (C:=t_unit); eauto.
+       forwards* : typing_regular Typ'.
+     }
+   * (*case typeofr*)
+     destruct H4.
+     apply inv_int in H5. destruct H5.
+     { (*case e = int*)
+      exists (open_ee e2 (e_lit i5)).
+      pick_fresh y.
+      assert (y \notin L) by auto.
+      lets: H1 y H6.
+      eapply step_typeofr with (C:=t_int); eauto.
+      forwards* : typing_regular Typ'.
+     }
+     { (*case e = \x.e*)
+      apply abs_typ_arrow_sub in H5.
+      destruct H5 as [A1 [B1]].
+      assert (sub (t_arrow t_top t_bot) (t_arrow A1 B1)) by auto.
+      eapply sub_transitivity in H5; eauto.
+      exists (open_ee e2 (e_abs e)).
+      pick_fresh y.
+      forwards*: H1 y.
+      eapply step_typeofr with (C:=(t_arrow t_top t_bot)); eauto.
+      forwards* : typing_regular Typ'.
+     }
+     { (*case e = null*)
+       apply inv_null in H5. destruct H5.
+       exists (open_ee e2 e_null).
+       pick_fresh y.
+       forwards*: H y.
+       eapply step_typeofr with (C:=t_unit); eauto.
+       forwards* : typing_regular Typ'.
+     }
+  + (*case typeof*)
+    destruct H4.
+    exists (e_typeof x A e1 B e2).
+    apply step_typeof; auto.
+    forwards* : typing_regular Typ'.
+  - forwards* : IHTyp1.
+Qed.
+
+(*******************************)
+(*****  Determinism Lemma  *****)
+(*******************************)
+
+Lemma inv_app : forall E e1 e2 A,
+typing E (e_app e1 e2) A ->
+exists A1 B1, typing E e1 (t_arrow A1 B1) /\ typing E e2 A1.
+Proof.
+  introv Typ.
+  inductions Typ.
+ - exists* A B.
+ - specialize (IHTyp e1 e2).
+  forwards* : IHTyp.
+ - forwards* : IHTyp1.
+Qed.
+
+Lemma inv_typeof : forall E e e1 e2 A B C,
+typing E (e_typeof e A e1 B e2) C ->
+exists D, typing E e D /\ A *s B.
+Proof.
+  introv Typ.
+  inductions Typ.
+  - specialize (IHTyp e e1 e2 A B).
+    forwards* : IHTyp.
+  - exists* (t_union A B).
+  - forwards* : IHTyp1.
+Qed.
+
+(********************************************)
+(** Value is normal form **)
+
+Lemma value_not_step : forall v e',
+  value v ->
+  step v e' -> False.
+Proof.
+  intros.
+  inverts H; try solve [inverts H0].
+Qed.
+
+(********************************************)
+(** findtype uniqueness **)
+
+Lemma findtype_unique : forall v A B,
+  findtype v A ->
+  findtype v B ->
+  A = B.
+Proof.
+  introv TypA TypB.
+  inverts TypA;
+  inverts* TypB.
+Qed.
+
+Lemma determinism : forall E e e1 e2 A, 
+  typing E e A ->
+  step e e1 -> step e e2 -> e1 = e2.
+Proof.
+  introv Typ He1. gen e2 A.
+  induction He1; introv Typ He2.
+  (*case step-appl*)
+  - inverts* He2.
+   + apply inv_app in Typ.
+     destruct Typ as [A1 [B1]]. destruct H0.
+     forwards* : IHHe1. rewrite* H3.
+   + inverts* H2; inverts He1.
+   + inverts* He1.
+(*case step-appr*)
+  - inverts* He2.
+   + inverts* H; inverts* H4.
+   + apply inv_app in Typ.
+     destruct Typ as [A1 [B1]]. destruct H0.
+     forwards* : IHHe1 H1. rewrite* H3.
+   + inverts H4; inverts He1.
+(*case step-beta*)
+  - inverts* He2.
+   + inverts* H5.
+   + inverts H0; inverts H5.
+(*case step-typeof*)
+ - inverts* He2.
+  + apply inv_typeof in Typ.
+    destruct Typ as [D]. destruct H0.
+    forwards* : IHHe1. rewrite* H2.
+  + inverts H8; inverts He1.
+  + inverts H8; inverts He1.
+(*case step-typeofl*)
+ - inverts* He2.
+  + apply value_not_step in H10; eauto.
+    inverts H10.
+  + apply inv_typeof in Typ.
+    destruct Typ as [D]. destruct H3 as [H3 Disj].
+    forwards*: findtype_unique H1 H11. subst.
+    forwards*: findtype_ord_type H1.
+    forwards*: sub_ord_disjoint_types Disj H2 H12.
+(*case step-typeofr*)
+- inverts* He2.
+  + inverts H0; inverts H10.
+  + apply inv_typeof in Typ.
+    destruct Typ as [D]. destruct H3 as [H3 Disj].
+    forwards*: findtype_unique H1 H11. subst.
+    forwards*: findtype_ord_type H1.
+    forwards*: sub_ord_disjoint_types Disj H12 H2.
+Qed.
