dockerfile
@@ -1,0 +1,48 @@
+FROM coqorg/coq:8.13.2 as  build
+LABEL maintainer="Baber Rehamn"
+
+RUN ["/bin/bash", "--login", "-c", "set -x \
+  && opam repository add --all-switches --set-default coq-released https://coq.inria.fr/opam/released"]
+
+# install coq TLC library
+
+RUN ["/bin/bash", "--login", "-c", "set -x \
+  && opam install -y coq-tlc.20210316"]
+  
+# install metalib/metatheory coq library
+
+RUN ["/bin/bash", "--login", "-c", "set -x \
+  && git clone https://github.com/plclub/metalib.git --branch coq8.10 --single-branch"]
+
+WORKDIR /home/coq/metalib/Metalib
+
+RUN ["/bin/bash", "--login", "-c", "set -x \
+  && make"]
+  
+RUN ["/bin/bash", "--login", "-c", "set -x \
+  && make install"]
+ 
+# copy coq code from local to docker image  
+  
+WORKDIR /home/coq
+
+RUN ["/bin/bash", "--login", "-c", "set -x \
+  && git clone https://github.com/baberrehman/phd-thesis-artifact.git"]
+
+#COPY --chown=coq code /home/coq/code
+
+# cleanup - delete unnecessary metalib files
+  
+RUN ["/bin/bash", "--login", "-c", "set -x \
+  && rm -r metalib"]
+  
+RUN ["/bin/bash", "--login", "-c", "set -x \
+  && sudo apt update -y"]
+  
+RUN ["/bin/bash", "--login", "-c", "set -x \
+  && sudo apt install vim -y"]
+
+#WORKDIR /home/coq/coq-duotyping/coq/DuoTyping
+
+#RUN ["/bin/bash", "--login", "-c", "set -x \
+#  && make"]
